clean up a bit

code/mpfr/MPFR.Lib.fst
@@ -79,27 +79,27 @@ type mpfr_reg_prec_t = p:u32{mpfr_PREC_COND (U32.v p)}
 type mpfr_reg_exp_t  = x:i32{mpfr_EXP_COND (I32.v x)}
 
 (* First bit is 1 *)
-let mpfr_d_valn_cond (m:mp_limb_t): GTot Type0 =
+inline_for_extraction let mpfr_d_valn_cond (m:mp_limb_t): GTot Type0 =
     v m >= pow2 63
 
 (* Ending bits are 0 *)
-let mpfr_d_val0_cond (m:mp_limb_t) (p:mpfr_prec_t{U32.v p > 0}): GTot Type0 =
+inline_for_extraction let mpfr_d_val0_cond (m:mp_limb_t) (p:mpfr_prec_t{U32.v p > 0}): GTot Type0 =
     v m % pow2 (prec_to_len (U32.v p) - U32.v p) = 0
 
-let normal_cond_ h (s:mpfr_struct): GTot Type0 =
+inline_for_extraction let normal_cond_ h (s:mpfr_struct): GTot Type0 =
     prec_to_len (U32.v s.mpfr_prec) = length s.mpfr_d * 64 /\
     mpfr_d_valn_cond (get h s.mpfr_d (length s.mpfr_d - 1)) /\
     mpfr_d_val0_cond (get h s.mpfr_d 0) s.mpfr_prec
 
-let normal_cond h (a:mpfr_ptr): GTot Type0 = normal_cond_ h (Seq.index (as_seq h a) 0)
+inline_for_extraction let normal_cond h (a:mpfr_ptr): GTot Type0 = normal_cond_ h (Seq.index (as_seq h a) 0)
 
-let mpfr_reg_cond_ h (s:mpfr_struct): GTot Type0 =
+inline_for_extraction let mpfr_reg_cond_ h (s:mpfr_struct): GTot Type0 =
     normal_cond_ h s /\
     mpfr_PREC_COND (U32.v s.mpfr_prec) /\ mpfr_EXP_COND (I32.v s.mpfr_exp)
 
-let mpfr_reg_cond h (a:mpfr_ptr): GTot Type0 = mpfr_reg_cond_ h (Seq.index (as_seq h a) 0)
+inline_for_extraction let mpfr_reg_cond h (a:mpfr_ptr): GTot Type0 = mpfr_reg_cond_ h (Seq.index (as_seq h a) 0)
 
-let mpfr_valid_cond_ h (s:mpfr_struct): GTot Type0 =
+inline_for_extraction let mpfr_valid_cond_ h (s:mpfr_struct): GTot Type0 =
     mpfr_PREC_COND (U32.v s.mpfr_prec) /\ 
     prec_to_len (U32.v s.mpfr_prec) = length s.mpfr_d * 64 /\
     (s.mpfr_exp = mpfr_EXP_NAN \/ s.mpfr_exp = mpfr_EXP_INF \/
@@ -222,39 +222,39 @@ let mpfr_modifies_trans_lemma a h0 h1 h2 = ()
 
 (* Access to entries *)
 (* precision *)
-val mpfr_PREC: x:mpfr_ptr -> Stack mpfr_prec_t 
+inline_for_extraction val mpfr_PREC: x:mpfr_ptr -> Stack mpfr_prec_t 
     (requires (fun h -> mpfr_live h x))
     (ensures  (fun h0 r h1 -> mpfr_live h1 x /\ h0 == h1 /\
                           r = (as_struct h1 x).mpfr_prec))
-let mpfr_PREC x = 
+inline_for_extraction let mpfr_PREC x = 
     let f = x.(0ul) in
     f.mpfr_prec
     
-val mpfr_GET_PREC: x:mpfr_ptr -> Stack mpfr_reg_prec_t 
+inline_for_extraction val mpfr_GET_PREC: x:mpfr_ptr -> Stack mpfr_reg_prec_t 
     (requires (fun h -> mpfr_live h x /\ mpfr_PREC_COND (U32.v (as_struct h x).mpfr_prec)))
     (ensures  (fun h0 r h1 -> mpfr_live h1 x /\ h0 == h1 /\
                           r = (as_struct h1 x).mpfr_prec))
-let mpfr_GET_PREC x = 
+inline_for_extraction let mpfr_GET_PREC x = 
     let f = x.(0ul) in
     f.mpfr_prec
 
 (* exponent *)
-val mpfr_EXP: x:mpfr_ptr -> Stack mpfr_exp_t 
+inline_for_extraction val mpfr_EXP: x:mpfr_ptr -> Stack mpfr_exp_t 
     (requires (fun h -> mpfr_live h x))
     (ensures  (fun h0 r h1 -> mpfr_live h1 x /\ h0 == h1 /\
                           r = (as_struct h1 x).mpfr_exp))
-let mpfr_EXP x = 
+inline_for_extraction let mpfr_EXP x = 
     let f = x.(0ul) in
     f.mpfr_exp
 
-val mpfr_SET_EXP: x:mpfr_ptr -> e:mpfr_exp_t -> Stack unit
+inline_for_extraction val mpfr_SET_EXP: x:mpfr_ptr -> e:mpfr_exp_t -> Stack unit
     (requires (fun h -> mpfr_live h x))
     (ensures  (fun h0 _ h1 -> mpfr_live h1 x /\ mpfr_modifies x h0 h1 /\
                            (as_struct h1 x).mpfr_exp = e /\
 			   (as_struct h1 x).mpfr_sign = (as_struct h0 x).mpfr_sign /\
 			   as_seq h1 (as_struct h1 x).mpfr_d == as_seq h0 (as_struct h0 x).mpfr_d))
 
-let mpfr_SET_EXP x e = 
+inline_for_extraction let mpfr_SET_EXP x e = 
     let h0 = ST.get() in
     let f = x.(0ul) in
     x.(0ul) <- {f with mpfr_exp = e};
@@ -262,31 +262,31 @@ let mpfr_SET_EXP x e =
     lemma_reveal_modifies_1 x h0 h1;
     lemma_intro_modifies_2 x (as_struct h1 x).mpfr_d h0 h1
 
-let mpfr_IS_NAN   x = mpfr_EXP x = mpfr_EXP_NAN
-let mpfr_SET_NAN  x = mpfr_SET_EXP x mpfr_EXP_NAN
-let mpfr_IS_INF   x = mpfr_EXP x = mpfr_EXP_INF
-let mpfr_SET_INF  x = mpfr_SET_EXP x mpfr_EXP_INF
-let mpfr_IS_ZERO  x = mpfr_EXP x = mpfr_EXP_ZERO
-let mpfr_SET_ZERO x = mpfr_SET_EXP x mpfr_EXP_ZERO
-let mpfr_NOTZERO  x = not (mpfr_IS_ZERO x)
+inline_for_extraction let mpfr_IS_NAN   x = mpfr_EXP x = mpfr_EXP_NAN
+inline_for_extraction let mpfr_SET_NAN  x = mpfr_SET_EXP x mpfr_EXP_NAN
+inline_for_extraction let mpfr_IS_INF   x = mpfr_EXP x = mpfr_EXP_INF
+inline_for_extraction let mpfr_SET_INF  x = mpfr_SET_EXP x mpfr_EXP_INF
+inline_for_extraction let mpfr_IS_ZERO  x = mpfr_EXP x = mpfr_EXP_ZERO
+inline_for_extraction let mpfr_SET_ZERO x = mpfr_SET_EXP x mpfr_EXP_ZERO
+inline_for_extraction let mpfr_NOTZERO  x = not (mpfr_IS_ZERO x)
 
 (* sign *)
-val mpfr_SIGN: x:mpfr_ptr -> Stack mpfr_sign_t 
+inline_for_extraction val mpfr_SIGN: x:mpfr_ptr -> Stack mpfr_sign_t 
     (requires (fun h -> mpfr_live h x))
     (ensures  (fun h0 r h1 -> mpfr_live h1 x /\ h0 == h1 /\
                            r = (as_struct h1 x).mpfr_sign))
-let mpfr_SIGN x = 
+inline_for_extraction let mpfr_SIGN x = 
     let f = x.(0ul) in
     f.mpfr_sign
 
-val mpfr_SET_SIGN: x:mpfr_ptr -> s:mpfr_sign_t -> Stack unit
+inline_for_extraction val mpfr_SET_SIGN: x:mpfr_ptr -> s:mpfr_sign_t -> Stack unit
     (requires (fun h -> mpfr_live h x))
     (ensures  (fun h0 _ h1 -> mpfr_live h1 x /\ mpfr_modifies x h0 h1 /\
                            (as_struct h1 x).mpfr_sign = s /\
 			   (as_struct h1 x).mpfr_exp = (as_struct h0 x).mpfr_exp /\
 			   as_seq h1 (as_struct h1 x).mpfr_d == as_seq h0 (as_struct h0 x).mpfr_d))
 			   
-let mpfr_SET_SIGN x s = 
+inline_for_extraction let mpfr_SET_SIGN x s = 
     let h0 = ST.get() in
     let f = x.(0ul) in
     x.(0ul) <- {f with mpfr_sign = s};
@@ -294,36 +294,36 @@ let mpfr_SET_SIGN x s =
     lemma_reveal_modifies_1 x h0 h1;
     lemma_intro_modifies_2 x (as_struct h1 x).mpfr_d h0 h1
 
-let mpfr_NEG_SIGN s = if s = mpfr_SIGN_POS then mpfr_SIGN_NEG else mpfr_SIGN_POS
+inline_for_extraction let mpfr_NEG_SIGN s = if s = mpfr_SIGN_POS then mpfr_SIGN_NEG else mpfr_SIGN_POS
 
-let mpfr_IS_POS x = I32.(mpfr_SIGN x >^ 0l)
-let mpfr_IS_NEG x = I32.(mpfr_SIGN x <^ 0l)
+inline_for_extraction let mpfr_IS_POS x = I32.(mpfr_SIGN x >^ 0l)
+inline_for_extraction let mpfr_IS_NEG x = I32.(mpfr_SIGN x <^ 0l)
 
-let mpfr_IS_STRICTPOS x = mpfr_NOTZERO x /\ mpfr_IS_POS x
-let mpfr_IS_STRICTNEG x = mpfr_NOTZERO x /\ mpfr_IS_NEG x
+inline_for_extraction let mpfr_IS_STRICTPOS x = mpfr_NOTZERO x /\ mpfr_IS_POS x
+inline_for_extraction let mpfr_IS_STRICTNEG x = mpfr_NOTZERO x /\ mpfr_IS_NEG x
 
-let mpfr_SET_POS x = mpfr_SET_SIGN x mpfr_SIGN_POS
-let mpfr_SET_NEG x = mpfr_SET_SIGN x mpfr_SIGN_NEG
+inline_for_extraction let mpfr_SET_POS x = mpfr_SET_SIGN x mpfr_SIGN_POS
+inline_for_extraction let mpfr_SET_NEG x = mpfr_SET_SIGN x mpfr_SIGN_NEG
 
-let mpfr_CHANGE_SIGN x = mpfr_SET_SIGN x (mpfr_NEG_SIGN (mpfr_SIGN x))
-let mpfr_SET_SAME_SIGN x y = mpfr_SET_SIGN x (mpfr_SIGN y)
-let mpfr_SET_OPPOSITE_SIGN x y = mpfr_SET_SIGN x (mpfr_NEG_SIGN (mpfr_SIGN y))
+inline_for_extraction let mpfr_CHANGE_SIGN x = mpfr_SET_SIGN x (mpfr_NEG_SIGN (mpfr_SIGN x))
+inline_for_extraction let mpfr_SET_SAME_SIGN x y = mpfr_SET_SIGN x (mpfr_SIGN y)
+inline_for_extraction let mpfr_SET_OPPOSITE_SIGN x y = mpfr_SET_SIGN x (mpfr_NEG_SIGN (mpfr_SIGN y))
 
-let mpfr_IS_POS_SIGN s = I32.(s >^ 0l)
-let mpfr_IS_NEG_SIGN s = I32.(s <^ 0l)
-let mpfr_MULT_SIGN (s1:mpfr_sign_t) (s2:mpfr_sign_t): Tot mpfr_sign_t  = I32.(s1 *^ s2)
+inline_for_extraction let mpfr_IS_POS_SIGN s = I32.(s >^ 0l)
+inline_for_extraction let mpfr_IS_NEG_SIGN s = I32.(s <^ 0l)
+inline_for_extraction let mpfr_MULT_SIGN (s1:mpfr_sign_t) (s2:mpfr_sign_t): Tot mpfr_sign_t  = I32.(s1 *^ s2)
 
 (* significand *)
-val mpfr_MANT: x:mpfr_ptr -> Stack (buffer mp_limb_t)
+inline_for_extraction val mpfr_MANT: x:mpfr_ptr -> Stack (buffer mp_limb_t)
     (requires (fun h -> mpfr_live h x))
     (ensures  (fun h0 r h1 -> mpfr_live h1 x /\ h0 == h1 /\
 			   r == (as_struct h1 x).mpfr_d))
 
-let mpfr_MANT x = 
+inline_for_extraction let mpfr_MANT x = 
     let f = x.(0ul) in
     f.mpfr_d
 
-val mpn_ZERO: b:buffer mp_limb_t -> l:u32 -> Stack unit
+inline_for_extraction val mpn_ZERO: b:buffer mp_limb_t -> l:u32 -> Stack unit
     (requires (fun h -> live h b /\ length b >= U32.v l))
     (ensures  (fun h0 _ h1 ->
         live h1 b /\ modifies_1 b h0 h1 /\
@@ -331,7 +331,7 @@ val mpn_ZERO: b:buffer mp_limb_t -> l:u32 -> Stack unit
         (forall (i:nat{i >= U32.v l /\ i < length b}). Seq.index (as_seq h1 b) i = Seq.index (as_seq h0 b) i) /\
         to_val (Seq.slice (as_seq h1 b) 0 (U32.v l)) = 0))
 
-let rec mpn_ZERO b l =
+inline_for_extraction let rec mpn_ZERO b l =
     if U32.(l =^ 0ul) then () else begin
         b.(U32.(l -^ 1ul)) <- 0uL;
         mpn_ZERO b U32.(l -^ 1ul);
@@ -340,43 +340,43 @@ let rec mpn_ZERO b l =
     end
 
 (* useful functions *)
-val mpfr_LAST_LIMB: x:mpfr_ptr -> Stack u32
+inline_for_extraction val mpfr_LAST_LIMB: x:mpfr_ptr -> Stack u32
     (requires (fun h -> mpfr_live h x /\ mpfr_PREC_COND (U32.v (as_struct h x).mpfr_prec)))
     (ensures  (fun h0 r h1 -> mpfr_live h1 x /\ h0 == h1 /\
                            (U32.v r + 1) * 64 = prec_to_len (U32.v (as_struct h1 x).mpfr_prec)))
 
-let mpfr_LAST_LIMB x =
+inline_for_extraction let mpfr_LAST_LIMB x =
     U32.((mpfr_GET_PREC x -^ 1ul) /^ gmp_NUMB_BITS)
 
-val mpfr_LIMB_SIZE: x:mpfr_ptr -> Stack u32
+inline_for_extraction val mpfr_LIMB_SIZE: x:mpfr_ptr -> Stack u32
     (requires (fun h -> mpfr_live h x /\ mpfr_PREC_COND (U32.v (as_struct h x).mpfr_prec)))
     (ensures  (fun h0 r h1 -> mpfr_live h1 x /\ h0 == h1 /\
                            U32.v r * 64 = prec_to_len (U32.v (as_struct h1 x).mpfr_prec)))
 
-let mpfr_LIMB_SIZE x = U32.(mpfr_LAST_LIMB x +^ 1ul)
+inline_for_extraction let mpfr_LIMB_SIZE x = U32.(mpfr_LAST_LIMB x +^ 1ul)
 
 (* special value *)
-let mpfr_LIMB_ONE = 1uL
+inline_for_extraction let mpfr_LIMB_ONE = 1uL
 
-val mpfr_LIMB_MASK: s:u32{U32.v s < 64} ->
+inline_for_extraction val mpfr_LIMB_MASK: s:u32{U32.v s < 64} ->
     Tot (r:u64{v r = pow2 (U32.v s) - 1})
-let mpfr_LIMB_MASK s =
+inline_for_extraction let mpfr_LIMB_MASK s =
     let lsh = 1uL <<^ s in
     lemma_pow2_small_mod (U32.v s) 64;
     lsh -^ 1uL
     
-val mpfr_LIMB_HIGHBIT: s:u64{v s = pow2 63}
-let mpfr_LIMB_HIGHBIT =
+inline_for_extraction val mpfr_LIMB_HIGHBIT: s:u64{v s = pow2 63}
+inline_for_extraction let mpfr_LIMB_HIGHBIT =
     assert_norm(UInt.pow2_n #64 63 = v 0x8000000000000000uL);
     0x8000000000000000uL
 
-val mpfr_LIMB_MAX: s:u64{v s = pow2 64 - 1}
-let mpfr_LIMB_MAX =
+inline_for_extraction val mpfr_LIMB_MAX: s:u64{v s = pow2 64 - 1}
+inline_for_extraction let mpfr_LIMB_MAX =
     assert_norm(pow2 64 - 1 = v 0xffffffffffffffffuL);
     0xffffffffffffffffuL
 
 (* set special value *)
-val mpfr_setmax_rec: x:mpfr_ptr -> i:u32 -> Stack unit
+inline_for_extraction val mpfr_setmax_rec: x:mpfr_ptr -> i:u32 -> Stack unit
     (requires (fun h -> 
         let p = (as_struct h x).mpfr_prec in
         mpfr_live h x /\ U32.v i < length (as_struct h x).mpfr_d /\ mpfr_PREC_COND (U32.v p)))
@@ -389,7 +389,7 @@ val mpfr_setmax_rec: x:mpfr_ptr -> i:u32 -> Stack unit
         v (Seq.index xm 0) = pow2 64 - pow2 (prec_to_len (U32.v p) - U32.v p) /\
         (forall (j:nat{j > 0 /\ j <= U32.v i}). v (Seq.index xm j) = pow2 64 - 1))))
 
-let rec mpfr_setmax_rec x i =
+inline_for_extraction let rec mpfr_setmax_rec x i =
     let mant = mpfr_MANT x in
     if i = 0ul then begin
         let p = mpfr_GET_PREC x in
@@ -425,7 +425,7 @@ let rec to_val_setmax_lemma s sh =
 	to_val_setmax_lemma (Seq.slice s 0 (Seq.length s - 1)) sh
     end
 
-val mpfr_setmax: x:mpfr_ptr -> Stack unit
+inline_for_extraction val mpfr_setmax: x:mpfr_ptr -> Stack unit
     (requires (fun h -> 
         let p = (as_struct h x).mpfr_prec in
         let l = U32.((p -^ 1ul) /^ 64ul +^ 1ul) in
@@ -437,7 +437,7 @@ val mpfr_setmax: x:mpfr_ptr -> Stack unit
 	as_reg_fp h1 x == mpfr_max_value (as_reg_fp h1 x).sign (as_reg_fp h1 x).prec /\
 	eval_abs (as_reg_fp h1 x) =. mpfr_overflow_bound (as_reg_fp h1 x).prec))
 
-let mpfr_setmax x =
+inline_for_extraction let mpfr_setmax x =
     mpfr_SET_EXP x mpfr_EMAX;
     mpfr_setmax_rec x (mpfr_LAST_LIMB x);
     let h = ST.get() in
@@ -467,7 +467,7 @@ let rec to_val_setmin_lemma s =
 	to_val_setmin_lemma (Seq.slice s 1 (Seq.length s))
     end
 
-val mpfr_setmin: x:mpfr_ptr -> Stack unit
+inline_for_extraction val mpfr_setmin: x:mpfr_ptr -> Stack unit
     (requires (fun h -> 
         let p = (as_struct h x).mpfr_prec in
         let l = U32.((p -^ 1ul) /^ 64ul +^ 1ul) in
@@ -479,7 +479,7 @@ val mpfr_setmin: x:mpfr_ptr -> Stack unit
 	as_reg_fp h1 x == mpfr_min_value (as_reg_fp h1 x).sign (as_reg_fp h1 x).prec /\
 	eval_abs (as_reg_fp h1 x) =. mpfr_underflow_bound (as_reg_fp h1 x).prec))
 
-let mpfr_setmin x =
+inline_for_extraction let mpfr_setmin x =
     mpfr_SET_EXP x mpfr_EMIN;
     let xn = mpfr_LAST_LIMB x in
     let xp = mpfr_MANT x in
